[Substitution]Unify unbox with unbox_fetch, here with get_here, letdia with letdia_get

label-free/Substitution.v
@@ -17,25 +17,25 @@ end.
    is ctx. *)
 Fixpoint subst_t_outer (M0: te_LF) (n: nat) (ctx: ctx_LF) (N0: te_LF) (curr: ctx_LF) {struct N0} :=
 match N0 with
-| hyp_LF n => hyp_LF n
-| lam_LF A M => lam_LF A (subst_t_outer M0 n ctx M curr)
-| appl_LF M N => appl_LF (subst_t_outer M0 n ctx M curr) (subst_t_outer M0 n ctx M curr)
+| hyp_LF n => 
+    hyp_LF n
+| lam_LF A M => 
+    lam_LF A (subst_t_outer M0 n ctx M curr)
+| appl_LF M N => 
+    appl_LF (subst_t_outer M0 n ctx M curr) (subst_t_outer M0 n ctx M curr)
 | box_LF M => 
   let w0 := var_gen (free_worlds_LF N0) in (* shouldn't we add sth? *)
     box_LF (subst_t_outer M0 n ctx M (fctx w0))
-| unbox_LF M => unbox_LF (subst_t_outer M0 n ctx M curr)
 | unbox_fetch_LF w M => 
   match (eq_ctx_LF_dec ctx w) with
     | left _ => unbox_fetch_LF w (subst_t_inner M0 n M ctx) 
     | right _ => unbox_fetch_LF w (subst_t_outer M0 n ctx M w)
   end
-| here_LF M => here_LF (subst_t_outer M0 n ctx M curr)
 | get_here_LF w M =>
   match (eq_ctx_LF_dec ctx w) with
     | left _ => get_here_LF w (subst_t_inner M0 n M ctx) 
     | right _ => get_here_LF w (subst_t_outer M0 n ctx M w)
   end
-| letdia_LF M N => letdia_LF (subst_t_outer M0 n ctx M curr) (subst_t_outer M0 n ctx N curr)
 | letdia_get_LF w M N =>
   match (eq_ctx_LF_dec ctx w) with
     | left _ => letdia_get_LF w (subst_t_inner M0 n M ctx) (subst_t_outer M0 n ctx N w)
@@ -45,25 +45,25 @@ end
 (* Current context is exactly the context in which we want to do susbtitution *)
 with subst_t_inner (M0: te_LF) (m: nat) (N0: te_LF) (curr: ctx_LF) {struct N0} :=
 match N0 with
-| hyp_LF n => if (eq_nat_dec n m) then M0 else hyp_LF n
-| lam_LF A M => lam_LF A (subst_t_inner M0 m M curr)
-| appl_LF M N => appl_LF (subst_t_inner M0 m M curr) (subst_t_inner M0 m N curr)
+| hyp_LF n => 
+    if (eq_nat_dec n m) then M0 else hyp_LF n
+| lam_LF A M => 
+    lam_LF A (subst_t_inner M0 m M curr)
+| appl_LF M N => 
+    appl_LF (subst_t_inner M0 m M curr) (subst_t_inner M0 m N curr)
 | box_LF M =>
   let w0 := var_gen (free_worlds_LF N0) in
     box_LF (subst_t_outer M0 m curr M (fctx w0))
-| unbox_LF M => unbox_LF (subst_t_inner M0 m M curr)
 | unbox_fetch_LF w M =>
   match (eq_ctx_LF_dec curr w) with
     | left _ => unbox_fetch_LF w (subst_t_inner M0 m M curr) 
     | right _ => unbox_fetch_LF w (subst_t_outer M0 m curr M w)
   end
-| here_LF M => here_LF (subst_t_inner M0 m M curr)
 | get_here_LF w M =>
   match (eq_ctx_LF_dec curr w) with
     | left _ => get_here_LF w (subst_t_inner M0 m M curr) 
     | right _ => get_here_LF w (subst_t_outer M0 m curr M w)
   end
-| letdia_LF M N => letdia_LF (subst_t_inner M0 m M curr) (subst_t_inner M0 m N curr)
 | letdia_get_LF w M N =>
   match (eq_ctx_LF_dec curr w) with
     | left _ => letdia_get_LF w (subst_t_inner M0 m M curr) (subst_t_outer M0 m curr N w)
@@ -72,7 +72,7 @@ match N0 with
 end.
 
 Definition subst_t M n ctx N curr :=
-  if (eq_ctx_LF_dec ctx curr) then (subst_t_inner M n N curr) 
+  If ctx = curr then (subst_t_inner M n N curr) 
   else (subst_t_outer M n ctx N curr). 
 
 Notation " [ M // n | ctx ] [ N | curr ] " := 
@@ -87,39 +87,95 @@ end.
 
 (* Context substitution *)
 
+Definition recalc_simpl_ctx (ctx:ctx_LF) : ctx_LF :=
+  match ctx with
+    | fctx _ => ctx
+    | bctx n => bctx (S n)
+end.
+
 Definition recalculate_ctx (ctx1: ctx_LF) (ctx2: ctx_LF) : prod ctx_LF ctx_LF :=
-   match ctx1, ctx2 with
-      | fctx w1', bctx w2' => (ctx1, bctx (S w2'))
-      | fctx w1', fctx w2' => (ctx1, ctx2)
-      | bctx w1', bctx w2' => (bctx (S w1'), bctx (S w2'))
-      | bctx w1', fctx w2' => (bctx (S w1'), ctx2)
-   end.
+  (recalc_simpl_ctx ctx1, recalc_simpl_ctx ctx2).
 
 (* We want to substitute ctx1 for every occ. of ctx2; our current context is curr.
    We assume in subst_ctx_outer that curr <> ctx2 *)
+
 (* len_old is used to calculate shift in new hypotheses, when we substitute for some bctx
    this should be set to 0 *)
 Fixpoint subst_ctx_outer (M0 : te_LF) (curr:ctx_LF) (ctx1: ctx_LF) (ctx2: ctx_LF) (len_old: nat) :=
 match M0 with 
 | hyp_LF n => hyp_LF n
+
 | lam_LF A M => lam_LF A (subst_ctx_outer M curr ctx1 ctx2 len_old)
+
 | appl_LF M N => appl_LF (subst_ctx_outer M curr ctx1 ctx2 len_old) 
                          (subst_ctx_outer N curr ctx1 ctx2 len_old)
 | box_LF M => 
-  let w0 := var_gen ((free_worlds_LF M) \u (var_from curr) \u (var_from ctx1) \u (var_from ctx2)) in
+  let w0 := var_gen (free_worlds_LF M) in
   let (ctx1', ctx2') := recalculate_ctx ctx1 ctx2 in 
     box_LF (subst_ctx_outer M (fctx w0) ctx1' ctx2' len_old)
-| unbox_LF M => unbox_LF (subst_ctx_outer M curr ctx1 ctx2 len_old)
+
+
+| unbox_fetch_LF w M => 
+  match (eq_ctx_LF_dec w ctx1) with
+  | left _ => unbox_fetch_LF ctx1 (subst_ctx_new M ctx1 ctx2 len_old)
+  | right _ =>
+    match (eq_ctx_LF_dec w ctx2) with
+    | left _ => unbox_fetch_LF ctx2 (subst_ctx_old M ctx1 ctx2 len_old)
+    | right _ => unbox_fetch_LF w (subst_ctx_outer M w ctx1 ctx2 len_old)
+    end
+  end
+
+| get_here_LF w M =>
+  match (eq_ctx_LF_dec w ctx1) with
+  | left _ => get_here_LF w (subst_ctx_new M ctx1 ctx2 len_old)
+  | right _ => 
+    match (eq_ctx_LF_dec w ctx2) with
+      | left _ => get_here_LF w (subst_ctx_old M ctx1 ctx2 len_old)
+      | right _ => get_here_LF w (subst_ctx_outer M w ctx1 ctx2 len_old)
+    end
+  end
+
+| letdia_get_LF w M N =>
+  let (ctx1', ctx2') := recalculate_ctx ctx1 ctx2 in
+  let curr' := recalc_simpl_ctx curr in
+  match (eq_ctx_LF_dec w ctx1) with
+  | left _ => letdia_get_LF w (subst_ctx_new M ctx1 ctx2 len_old) 
+                              (subst_ctx_outer N curr' ctx1' ctx2' len_old)
+  | right _ => 
+    match (eq_ctx_LF_dec w ctx2) with
+    | left _ => letdia_get_LF w (subst_ctx_old M ctx1 ctx2 len_old) 
+                                (subst_ctx_outer N curr' ctx1' ctx2' len_old)
+    | right _ => 
+          letdia_get_LF w (subst_ctx_outer M w ctx1 ctx2 len_old)  
+                          (subst_ctx_outer N curr' ctx1' ctx2' len_old)
+    end
+  end
+end
+(* In subst_ctx_old we assume that current context was ctx2, now changed to ctx1 *)
+with subst_ctx_old (M0 : te_LF) (ctx1: ctx_LF) (ctx2: ctx_LF) (len_old: nat) :=
+match M0 with 
+| hyp_LF n => hyp_LF n
+
+| lam_LF A M => lam_LF A (subst_ctx_old M ctx1 ctx2 (len_old))
+
+| appl_LF M N => appl_LF (subst_ctx_old M ctx1 ctx2 len_old) 
+                         (subst_ctx_old N ctx1 ctx2 len_old)
+
+| box_LF M =>
+  let w0 := var_gen (free_worlds_LF M \u (var_from ctx1) \u (var_from ctx2)) in
+  let (ctx1', ctx2') := recalculate_ctx ctx1 ctx2 in     
+    box_LF (subst_ctx_outer M (fctx w0) ctx1' ctx2' len_old)
+
 | unbox_fetch_LF w M =>
   match (eq_ctx_LF_dec w ctx1) with
   | left _ => unbox_fetch_LF w (subst_ctx_new M ctx1 ctx2 len_old)
   | right _ => 
-    match (eq_ctx_LF_dec w ctx2) with
+    match (eq_ctx_LF_dec w ctx2) with 
       | left _ => unbox_fetch_LF w (subst_ctx_old M ctx1 ctx2 len_old)
       | right _ => unbox_fetch_LF w (subst_ctx_outer M w ctx1 ctx2 len_old)
     end
-   end
-| here_LF M => here_LF (subst_ctx_outer M curr ctx1 ctx2 len_old)
+  end 
+
 | get_here_LF w M =>
   match (eq_ctx_LF_dec w ctx1) with
   | left _ => get_here_LF w (subst_ctx_new M ctx1 ctx2 len_old)
@@ -129,88 +185,49 @@ match M0 with
       | right _ => get_here_LF w (subst_ctx_outer M w ctx1 ctx2 len_old)
     end
    end
-| letdia_LF M N =>
-  let (ctx1', ctx2') := recalculate_ctx ctx1 ctx2 in 
-    letdia_LF (subst_ctx_outer M curr ctx1 ctx2 len_old)
-              (subst_ctx_outer N curr ctx1' ctx2' len_old)
+
 | letdia_get_LF w M N =>
-  let (ctx1', ctx2') := recalculate_ctx ctx1 ctx2 in 
+  let (ctx1', ctx2') := recalculate_ctx ctx1 ctx2 in
+  let N' := subst_ctx_old N ctx1' ctx2' len_old in
   match (eq_ctx_LF_dec w ctx1) with
-  | left _ => letdia_get_LF w (subst_ctx_new M ctx1 ctx2 len_old) 
-                              (subst_ctx_outer N curr ctx1' ctx2' len_old)
-  | right _ => 
+  | left _ => letdia_get_LF w (subst_ctx_new M ctx1 ctx2 len_old) N'
+  | right _ =>
     match (eq_ctx_LF_dec w ctx2) with
-      | left _ => letdia_get_LF w (subst_ctx_old M ctx1 ctx2 len_old) 
-                                  (subst_ctx_outer N curr ctx1' ctx2' len_old)
-      | right _ => letdia_get_LF w (subst_ctx_outer M w ctx1 ctx2 len_old) 
-                                   (subst_ctx_outer N curr ctx1' ctx2' len_old)
-    end
-   end
-end
-(* In subst_ctx_old we assume that current context is ctx2 *)
-with subst_ctx_old (M0 : te_LF) (ctx1: ctx_LF) (ctx2: ctx_LF) (len_old: nat) :=
-match M0 with 
-| hyp_LF n => hyp_LF n
-| lam_LF A M => lam_LF A (subst_ctx_old M ctx1 ctx2 (len_old))
-| appl_LF M N => appl_LF (subst_ctx_old M ctx1 ctx2 len_old) 
-                         (subst_ctx_old N ctx1 ctx2 len_old)
-| box_LF M =>
-  let w0 := var_gen (free_worlds_LF M \u (var_from ctx1) \u (var_from ctx2)) in
-  let (ctx1', ctx2') := recalculate_ctx ctx1 ctx2 in     
-    box_LF (subst_ctx_outer M (fctx w0) ctx1' ctx2' len_old)
-| unbox_LF M => unbox_LF (subst_ctx_old M ctx1 ctx2 len_old)
-| unbox_fetch_LF w M =>
-  match (eq_ctx_LF_dec w ctx1) with
-  | left _ => unbox_fetch_LF ctx1 (subst_ctx_new M ctx1 ctx2 len_old)
-  | right _ => unbox_fetch_LF w (subst_ctx_outer M w ctx1 ctx2 len_old)
-   end
-| here_LF M => here_LF (subst_ctx_old M ctx1 ctx2 len_old)
-| get_here_LF w M =>
-  match (eq_ctx_LF_dec w ctx1) with
-  | left _ => get_here_LF ctx1 (subst_ctx_new M ctx1 ctx2 len_old)
-  | right _ => 
-    match (eq_ctx_LF_dec w ctx2) with
-      | left _ => get_here_LF w (subst_ctx_old M ctx1 ctx2 len_old)
-      | right _ => get_here_LF w (subst_ctx_outer M w ctx1 ctx2 len_old)
-    end
-   end
-| letdia_LF M N => 
-  let (ctx1', ctx2') := recalculate_ctx ctx1 ctx2 in 
-    letdia_LF (subst_ctx_old M ctx1 ctx2 len_old) 
-              (subst_ctx_old N ctx1' ctx2' len_old)
-| letdia_get_LF w M N =>
-  let (ctx1', ctx2') := recalculate_ctx ctx1 ctx2 in 
-  match (eq_ctx_LF_dec w ctx1) with
-  | left _ => letdia_get_LF ctx1 (subst_ctx_new M ctx1 ctx2 len_old) (subst_ctx_old M ctx1' ctx2' len_old)
-  | right _ => 
-    match (eq_ctx_LF_dec w ctx2) with
-      | left _ => letdia_get_LF w (subst_ctx_old M ctx1 ctx2 len_old) (subst_ctx_old M ctx1' ctx2' len_old) 
-      | right _ => letdia_get_LF w (subst_ctx_outer M w ctx1 ctx2 len_old) (subst_ctx_old M ctx1' ctx2' len_old) 
+    | left _ => letdia_get_LF w (subst_ctx_old M ctx1 ctx2 len_old) N'
+    | right _ => letdia_get_LF w (subst_ctx_outer M w ctx1 ctx2 len_old) N'
     end
   end
 end
 (* In subst_ctx_new we assume that current context is ctx1 *)
 with subst_ctx_new (M0 : te_LF) (ctx1: ctx_LF) (ctx2: ctx_LF) (len_old: nat) :=
 match M0 with 
+
 | hyp_LF n => 
   match ctx2 with
     | bctx _ => hyp_LF n
     | fctx _ => hyp_LF (len_old+n)
   end
+
 | lam_LF A M => lam_LF A (subst_ctx_new M ctx1 ctx2 len_old)
+
 | appl_LF M N => appl_LF (subst_ctx_new M ctx1 ctx2 len_old) 
                          (subst_ctx_new N ctx1 ctx2 len_old)
+
 | box_LF M =>
   let w0 := var_gen (free_worlds_LF M \u (var_from ctx1) \u (var_from ctx2)) in
   let (ctx1', ctx2') := recalculate_ctx ctx1 ctx2 in 
     box_LF (subst_ctx_outer M (fctx w0) ctx1' ctx2' len_old)
-| unbox_LF M => unbox_LF (subst_ctx_new M ctx1 ctx2 len_old)
+
 | unbox_fetch_LF w M =>
   match (eq_ctx_LF_dec w ctx2) with
-    | left _ => unbox_fetch_LF ctx1 (subst_ctx_old M ctx1 ctx2 len_old)
-    | right _ => unbox_fetch_LF w (subst_ctx_outer M w ctx1 ctx2 len_old)
+    | left _ => unbox_fetch_LF w (subst_ctx_old M ctx1 ctx2 len_old)
+    | right _ => 
+      match (eq_ctx_LF_dec w ctx2) with 
+        | left _ => unbox_fetch_LF ctx1 (subst_ctx_old M ctx1 ctx2 len_old)
+        | right _ => unbox_fetch_LF w (subst_ctx_outer M w ctx1 ctx2 len_old)
+      end
   end
-| here_LF M => here_LF (subst_ctx_new M ctx1 ctx2 len_old)
+
 | get_here_LF w M =>
   match (eq_ctx_LF_dec w ctx1) with
   | left _ => get_here_LF w (subst_ctx_new M ctx1 ctx2 len_old)
@@ -220,29 +237,34 @@ match M0 with
       | right _ => get_here_LF w (subst_ctx_outer M w ctx1 ctx2 len_old)
     end
    end
-| letdia_LF M N => 
-  let (ctx1', ctx2') := recalculate_ctx ctx1 ctx2 in 
-    letdia_LF (subst_ctx_new M ctx1 ctx2 len_old) 
-              (subst_ctx_new N ctx1' ctx2' len_old)
+
 | letdia_get_LF w M N =>
-  let (ctx1', ctx2') := recalculate_ctx ctx1 ctx2 in 
+  let (ctx1', ctx2') := recalculate_ctx ctx1 ctx2 in
   match (eq_ctx_LF_dec w ctx1) with
-  | left _ => letdia_get_LF w (subst_ctx_new M ctx1 ctx2 len_old) (subst_ctx_old M ctx1' ctx2' len_old)
-  | right _ => 
+  | left _ => letdia_get_LF w (subst_ctx_new M ctx1 ctx2 len_old) 
+                              (subst_ctx_old N ctx1' ctx2' len_old)
+  | right _ =>
     match (eq_ctx_LF_dec w ctx2) with
-      | left _ => letdia_get_LF ctx1 (subst_ctx_old M ctx1 ctx2 len_old) (subst_ctx_old M ctx1' ctx2' len_old) 
-      | right _ => letdia_get_LF w (subst_ctx_outer M w ctx1 ctx2 len_old) (subst_ctx_old M ctx1' ctx2' len_old) 
+      | left _ => letdia_get_LF ctx1 (subst_ctx_old M ctx1 ctx2 len_old) 
+                                     (subst_ctx_old N ctx1' ctx2' len_old) 
+      | right _ => letdia_get_LF w (subst_ctx_outer M w ctx1 ctx2 len_old) 
+                                   (subst_ctx_old N ctx1' ctx2' len_old) 
     end
-  end
+  end 
 end.
 
 Definition subst_ctx M c1 c2 curr len_old :=
 match (eq_ctx_LF_dec c1 c2) with
 | left _ => M
 | right _ => 
-  if (eq_ctx_LF_dec curr c1) then subst_ctx_new M c1 c2 len_old
-  else if (eq_ctx_LF_dec curr c2) then subst_ctx_old M c1 c2 len_old
-       else subst_ctx_outer M curr c1 c2 len_old
+  match (eq_ctx_LF_dec curr c1) with
+  | left _ => subst_ctx_new M c1 c2 len_old
+  | right _ => 
+    match (eq_ctx_LF_dec curr c2) with
+    | left _ => subst_ctx_old M c1 c2 len_old
+    | right _ => subst_ctx_outer M curr c1 c2 len_old
+    end
+  end
 end.
 
 Notation " {{ c1 // c2 }} [ M | curr , m ] " := 
@@ -288,232 +310,19 @@ reflexivity.
 Qed.
 
 
-(*
-Lemma no_unbound_worlds_subst_w_id:
-forall M w k w'
-  (H_unbound: unbound_worlds k M = nil),
-  {{w//bctx k}}[M | w', 0] = M.
-intros;
-generalize dependent w;
-generalize dependent k;
-induction M; unfold subst_ctx in *;
-intros.
-(* hyp *)
-repeat case_if; reflexivity.
-(* lam *)
-apply IHM with (w:=w) in H_unbound;
-repeat case_if; simpl;
-try rewrite H_unbound; reflexivity.
-(* appl *)
-simpl in H_unbound;
-apply app_eq_nil in H_unbound;
-destruct H_unbound as (H_Un1, H_Un2);
-apply IHM1 with (w:=w) in H_Un1;
-apply IHM2 with (w:=w) in H_Un2;
-repeat case_if; simpl;
-try (rewrite H_Un1; rewrite H_Un2); reflexivity.
-(* box *)
-
+Lemma subst_ctx_rewrite_new:
+forall w0 w1 k M, 
+  {{ w0 // w1}}[ {{w1 // k}} [M | w1, 0] | w1, 0] = {{ w0 // k }} [M | w0, 0]. 
 Admitted.
 
-Lemma closed_w_subst_id:
-forall M w n w'
-  (HT: lc_w_n_LF M n),
-  {{w//bctx n}} [M | w', 0] = M.
-intros;
-apply no_unbound_worlds_subst_w_id;
-apply closed_no_unbound_worlds;
-assumption.
-Qed.
-
-Lemma subst_order_irrelevant:
-forall N M n m w w' w''
-  (H_LC: lc_w_LF M),
-  subst_ctx ([M//n | w''] [N | w']) w (bctx m) w' 0 = 
-  [M//n | w''] [(subst_ctx N w (bctx m) w' 0) | w'].
+Lemma subst_ctx_rewrite_old:
+forall w0 w1 k M, 
+  {{ w0 // w1}}[ {{w1 // k}} [M | w1, 0] | w1, 0] = {{ w0 // k }} [M | w0, 0]. 
 Admitted.
 
-Lemma subst_w_comm:
-forall M w w' w'' n w0 w1 k
-  (Neq: w'' <> w),
-  {{fctx w'//fctx w''}}[({{fctx w//bctx n}}[M | w0, 0]) | w1, k] = {{fctx w//bctx n}}[({{fctx w'//fctx w''}}[M | w1, k]) | w0, 0].
-Admitted.
-*)
-
-Lemma var_gen_neq:
-  forall w S
-  (HT: w \in S),
-  fctx w <> fctx (var_gen S).
-intros; intro; inversion H; subst;
-assert (var_gen S \notin S) by apply var_gen_spec;
-contradiction.
-Qed.
-
-Ltac in_singleton_union :=
-match goal with
-| |- ?w \in \{?w} => rewrite in_singleton; reflexivity
-| |- ?w \in \{?w} \/ _ => left; in_singleton_union
-| |- _ \/ ?w \in \{?w} => right; in_singleton_union
-| |- _ \/ ?w \in \{?w} \/ _ => right; in_singleton_union
-| |- _ \/ _ \/ ?w \in \{?w}  => right; in_singleton_union
-| _ => fail
-end.
-
-Ltac autorewrite_ctx :=
-match goal with 
-| [H : (bctx ?n = bctx ?n') |- _ ] => rewrite H
-| [H : (fctx ?n = fctx ?n') |- _ ] => rewrite H
-| _ => skip
-end.
-
-Lemma subst_id:
-forall M w n w0 w0' k
-  (HT: w \notin (free_worlds_LF M)),
-  {{bctx n // fctx w}}[ {{fctx w // bctx n}} [M | fctx w0', 0] | fctx w0, k] = M.
-intros;
-generalize dependent n;
-generalize dependent w0';
-generalize dependent w0;
-induction M; intros.
-(* hyp *)
-unfold subst_ctx;
-simpl in *;
-repeat case_if;
-reflexivity.
-(* lam *)
-simpl in HT;
-unfold subst_ctx;
-repeat case_if; 
-subst; simpl in *;
-try repeat rewrite subst_ctx__new;
-try repeat rewrite subst_ctx__old;
-try repeat rewrite subst_ctx__outer;
-auto;
-rewrite IHM; auto.
-(* appl *)
-simpl in HT; rewrite notin_union in HT; destruct HT;
-unfold subst_ctx;
-repeat case_if;
-subst; simpl in *;
-try repeat rewrite subst_ctx__new;
-try repeat rewrite subst_ctx__old;
-try repeat rewrite subst_ctx__outer;
-auto;
-try rewrite IHM1; try rewrite IHM2; auto.
-(* box *)
-simpl in HT;
-unfold subst_ctx;
-repeat case_if;
-subst; simpl in *;
-try repeat rewrite subst_ctx__outer;
-try rewrite IHM; 
-try discriminate;
-try (apply var_gen_neq;
-  repeat rewrite in_union; right; 
-  in_singleton_union);
-auto.
-(* unbox *)
-simpl in HT;
-unfold subst_ctx;
-repeat case_if;
-subst; simpl in *;
-try repeat rewrite subst_ctx__new;
-try repeat rewrite subst_ctx__old;
-try repeat rewrite subst_ctx__outer;
-try rewrite IHM; 
-try discriminate;
-auto.
-(* unbox_fetch *)
-simpl in HT; destruct c; simpl in HT;
-try (rewrite notin_union in HT; destruct HT);
-unfold subst_ctx;
-repeat (case_if; simpl);
-subst; simpl in *;
-try repeat rewrite subst_ctx__new;
-try repeat rewrite subst_ctx__old;
-try repeat rewrite subst_ctx__outer;
-try rewrite IHM; 
-autorewrite_ctx;
-try discriminate;
-auto;
-autorewrite_ctx.
-(* here *)
-simpl in HT;
-unfold subst_ctx;
-repeat case_if;
-subst; simpl in *;
-try repeat rewrite subst_ctx__new;
-try repeat rewrite subst_ctx__old;
-try repeat rewrite subst_ctx__outer;
-try rewrite IHM; 
-try discriminate;
-auto.
-(* get_here *)
-simpl in HT; destruct c; simpl in HT;
-try (rewrite notin_union in HT; destruct HT);
-unfold subst_ctx;
-repeat (case_if; simpl);
-subst; simpl in *;
-try repeat rewrite subst_ctx__new;
-try repeat rewrite subst_ctx__old;
-try repeat rewrite subst_ctx__outer;
-try rewrite IHM; 
-autorewrite_ctx;
-try discriminate;
-auto;
-autorewrite_ctx.
-(* letdia *)
-simpl in HT;
-unfold subst_ctx;
-repeat case_if;
-subst; simpl in *;
-try repeat rewrite subst_ctx__new;
-try repeat rewrite subst_ctx__old;
-try repeat rewrite subst_ctx__outer;
-try rewrite IHM1;
-try rewrite IHM2; 
-try discriminate;
-auto.
-(* letdia_get *)
-simpl in HT; destruct c; simpl in HT;
-try (rewrite notin_union in HT; destruct HT);
-unfold subst_ctx;
-repeat (case_if; simpl);
-subst; simpl in *;
-try repeat rewrite subst_ctx__new;
-try repeat rewrite subst_ctx__old;
-try repeat rewrite subst_ctx__outer;
-try rewrite IHM1;
-try rewrite IHM2; 
-autorewrite_ctx;
-try discriminate;
-auto;
-autorewrite_ctx.
-Qed.
-
-(* This is just one option of neutral substitution! *)
-Lemma subst_neutral:
-forall M w w' n k
-  (HT: lc_w_n_LF M n),
-  {{fctx w//bctx n}}[({{bctx n//fctx w'}}[M | fctx w', k]) | fctx w, 0] = {{fctx w//fctx w'}}[ M | fctx w', k].
-Admitted.
-
-Lemma subst_neutral':
-forall M w w' n  k
-  (HT: lc_w_n_LF M n),
-  {{fctx w//bctx n}}[({{bctx n//fctx w'}}[M | fctx w, k]) | fctx w, 0] = {{fctx w//fctx w'}}[ M | fctx w, k].
-Admitted.
-
-Lemma subst_neutral'':
-forall M w w' w0 n  k
-  (HT: lc_w_n_LF M n),
-  {{fctx w//bctx n}}[({{bctx n//fctx w'}}[M | fctx w0, k]) | fctx w0, 0] = {{fctx w//fctx w'}}[ M | fctx w0, k].
-Admitted.
-
-Lemma closed_step_opening:
-forall M n w w0
-  (HT: lc_w_n_LF M (S n)),
-  lc_w_n_LF ({{fctx w//bctx n}}[M | w0, 0]) n.
+Lemma subst_ctx_rewrite_outer:
+forall w0 w1 w k l M, 
+  {{ w0 // w1}}[ {{w1 // k}} [M | w, 0] | w, l] = {{ w0 // k }} [M | w, 0]. 
 Admitted.
 
 End Lemmas.
